Put map structure into global ghost state,
proved laws for ghost ownership. This is probably the version that I'll
try to push through veric.

veric/own.v
@@ -7,9 +7,11 @@ Require Import VST.veric.res_predicates.
 Import RML. Import R.
 Local Open Scope pred.
 
+Notation ghost_approx m := (ghost_fmap (approx (level m)) (approx (level m))).
+
 (* Ghost state construction drawn from "Iris from the ground up", Jung et al. *)
 Program Definition ghost_is (g : ghost): pred rmap :=
-  fun m => ghost_of m = ghost_fmap (approx (level m)) (approx (level m)) g.
+  fun m => ghost_of m = ghost_approx m g.
 Next Obligation.
   repeat intro.
   erewrite (age1_ghost_of _ _ H) by (symmetry; apply ghost_of_approx).
@@ -25,12 +27,12 @@ Lemma Own_op: forall {RA: Ghost} (a b c: ghost), join a b c ->
 Proof.
   intros; apply pred_ext.
   - intros w [Hno Hg]; simpl in *.
-    destruct (make_rmap (resource_at w) (ghost_fmap (approx (level w)) (approx (level w)) a)
-      (rmap_valid w) (level w)) as (wa & Hla & Hra & Hga).
+    destruct (make_rmap (resource_at w) (ghost_approx w a) (rmap_valid w) (level w))
+      as (wa & Hla & Hra & Hga).
     { extensionality; apply resource_at_approx. }
     { rewrite ghost_fmap_fmap, approx_oo_approx; auto. }
-    destruct (make_rmap (resource_at w) (ghost_fmap (approx (level w)) (approx (level w)) b)
-      (rmap_valid w) (level w)) as (wb & Hlb & Hrb & Hgb).
+    destruct (make_rmap (resource_at w) (ghost_approx w b) (rmap_valid w) (level w))
+      as (wb & Hlb & Hrb & Hgb).
     { extensionality; apply resource_at_approx. }
     { rewrite ghost_fmap_fmap, approx_oo_approx; auto. }
     exists wa, wb; rewrite Hla, Hlb, Hra, Hrb; split; auto.
@@ -51,23 +53,50 @@ Proof.
 Qed.
 
 Program Definition bupd (P: pred rmap): pred rmap :=
-  fun m => forall c, joins (ghost_of m) c -> exists b, joins b c /\ exists m',
-    level m' = level m /\ resource_at m' = resource_at m /\ ghost_of m' = b /\ P m'.
+  fun m => forall c, joins (ghost_of m) (ghost_approx m c) ->
+    exists b, joins b (ghost_approx m c) /\
+    exists m', level m' = level m /\ resource_at m' = resource_at m /\ ghost_of m' = b /\ P m'.
 Next Obligation.
 Proof.
   repeat intro.
   erewrite (age1_ghost_of _ _ H) in H1 by (symmetry; apply ghost_of_approx).
-  destruct (ghost_of a) eqn: Hga; simpl in *.
-  destruct H1 as [d H1]; inv H1.
-  inj_pair_tac.
-  destruct (H0 (GHOST _ b pds)) as (b' & J' & Hrb).
-  { eexists; constructor; eauto. }
-  destruct b', J' as [? J']; inv J'.
-  repeat inj_pair_tac.
-  exists (GHOST _ g0 (preds_fmap (approx (level a')) (approx (level a')) pds)); split.
-  - eexists; constructor; eauto.
+  rewrite <- ghost_of_approx in H0.
+  destruct (ghost_of a) as [?? ga pdsa], c as [?? gc pdsc], H1 as [? H1]; inv H1; repeat inj_pair_tac.
+  assert (forall i n pp, match pdsa i n, pdsc i n with Some x, Some _ => Some x | _, _ => pdsc i n end = Some pp ->
+    exists a, finmap_get (gc i) n = Some a) as dom'.
+  { intros; destruct (pdsa i n) eqn: Hi; eauto.
+    destruct (pdsc i n) eqn: Hi'; inv H1; eauto. }
+  specialize (H0 (GHOST _ _ gc _ dom')); destruct H0 as (b & J & Hrb).
+  { eexists; constructor; eauto.
+    instantiate (1 := fun i n => option_map (preds_fmap (approx (level a)) (approx (level a)))
+      match pdsa i n with Some x => Some x | _ => pdsc i n end).
+    intros i n; specialize (H12 i n); inv H12.
+    * destruct (pdsa i n); inv H1; constructor.
+    * destruct (pdsc i n); inv H2.
+      destruct (pdsa i n); constructor; auto.
+    * destruct (pdsa i n); inv H0.
+      destruct (pdsc i n); inv H1.
+      inv H3; constructor; auto. }
+  pose proof (age_level _ _ H).
+  exists (ghost_approx a' b); split.
+  - destruct b as [?? gb pdsb]; destruct J as [? J]; inv J; repeat inj_pair_tac.
+    eexists; constructor; eauto.
+    instantiate (1 := fun i n => option_map (preds_fmap (approx (level a')) (approx (level a')))
+      match pdsb i n with Some x => Some x | _ => pdsc i n end).
+    intros i n; specialize (H12 i n); specialize (H13 i n); inv H13; simpl; try constructor.
+    + assert (pdsc i n = None) as ->.
+      { destruct (pdsa i n), (pdsc i n); auto; inv H3. }
+      destruct (pdsb i n); constructor.
+    + inv H12; try constructor.
+      * destruct (pdsa i n); inv H6.
+        destruct (pdsc i n); inv H2.
+        inv H4; constructor.
+        rewrite preds_fmap_fmap, approx_oo_approx', approx'_oo_approx by omega; auto.
+      * destruct (pdsa i n); inv H5.
+        destruct (pdsc i n); inv H6.
+        inv H2; inv H4; inv H8.
+        rewrite <- H2, preds_fmap_fmap, approx_oo_approx', approx'_oo_approx by omega; auto.
   - destruct Hrb as (m' & Hl' & Hr' & Hg' & HP).
-    pose proof (age_level _ _ H).
     destruct (levelS_age m' (level a')) as (m'' & Hage' & Hl'').
     { congruence. }
     exists m''; repeat split; auto.
@@ -78,45 +107,48 @@ Proof.
     + erewrite (age1_ghost_of _ _ Hage') by (symmetry; apply ghost_of_approx).
       rewrite Hg', Hl''; auto.
     + eapply (proj2_sig P); eauto.
+  Unshelve.
+  simpl; intros.
+  specialize (H11 i); apply finmap_get_join with (i0 := n) in H11.
+  destruct (finmap_get (c0 i) n); eauto.
+  destruct (pdsa i n) eqn: Hi; inv H0.
+  destruct (dom _ _ _ Hi) as [? Hget]; rewrite Hget in H11.
+  destruct (finmap_get (gc i) n); inv H11.
+  destruct (pdsc i n) eqn: Hi'; inv H2.
+  destruct (dom0 _ _ _ Hi') as [? Hget]; rewrite Hget in H11.
+  destruct (finmap_get (ga i) n); inv H11.
+  simpl; intros.
+  specialize (H10 i); apply finmap_get_join with (i0 := n) in H10.
+  destruct (finmap_get (c1 i) n); eauto.
+  destruct (pdsb i n) eqn: Hi; inv H0.
+  destruct (dom1 _ _ _ Hi) as [? Hget]; rewrite Hget in H10.
+  destruct (finmap_get (gc i) n); inv H10.
+  destruct (pdsc i n) eqn: Hi'; inv H1.
+  destruct (dom0 _ _ _ Hi') as [? Hget]; rewrite Hget in H10.
+  destruct (finmap_get (gb i) n); inv H10.
 Qed.
 
-Definition fp_update (a b : ghost) :=
-  forall n c, joins (ghost_fmap (approx n) (approx n) a) c ->
-               joins (ghost_fmap (approx n) (approx n) b) c.
-
-Lemma Own_update: forall a b, fp_update a b ->
-  Own a |-- bupd (Own b).
+Lemma bupd_mono: forall P Q, P |-- Q -> bupd P |-- bupd Q.
 Proof.
   repeat intro.
-  destruct H0 as [Hno Hg]; simpl in *.
-  rewrite Hg in H1.
-  destruct H1 as [? J].
-  destruct (H (level a0) c).
-  { eexists; eauto. }
-  exists (ghost_fmap (approx (level a0)) (approx (level a0)) b); split.
-  { eexists; eauto. }
-  destruct (make_rmap (resource_at a0)
-    (ghost_fmap (approx (level a0)) (approx (level a0)) b) (rmap_valid a0) (level a0))
-    as (m' & Hl & Hr & ?).
-  { extensionality; apply resource_at_approx. }
-  { rewrite ghost_fmap_fmap, approx_oo_approx; auto. }
+  simpl in *.
+  destruct (H0 _ H1) as (b & ? & m' & ? & ? & ? & ?).
+  exists b; split; auto.
   exists m'; repeat split; auto.
-  - intro; rewrite Hr; auto.
-  - rewrite Hl; auto.
 Qed.
 
-Definition fp_update_ND a B :=
+Definition ghost_fp_update_ND a B :=
   forall n c, joins (ghost_fmap (approx n) (approx n) a) c ->
     exists b, B b /\ joins (ghost_fmap (approx n) (approx n) b) c.
 
-Lemma Own_update_ND: forall {RA: Ghost} a B, fp_update_ND a B ->
+Lemma Own_update_ND: forall a B, ghost_fp_update_ND a B ->
   Own a |-- bupd (EX b : _, !!(B b) && Own b).
 Proof.
   repeat intro.
   destruct H0 as [Hno Hg]; simpl in *.
   rewrite Hg in H1.
   destruct H1 as [? J].
-  destruct (H (level a0) c) as (g' & ? & ?).
+  destruct (H (level a0) (ghost_approx a0 c)) as (g' & ? & ?).
   { eexists; eauto. }
   exists (ghost_fmap (approx (level a0)) (approx (level a0)) g'); split; auto.
   destruct (make_rmap (resource_at a0)
@@ -130,49 +162,312 @@ Proof.
   - rewrite Hl; auto.
 Qed.
 
-Definition gname := nat.
+Definition ghost_fp_update (a b : ghost) :=
+  forall n c, joins (ghost_fmap (approx n) (approx n) a) c ->
+               joins (ghost_fmap (approx n) (approx n) b) c.
 
-(* Note that finite maps are not a Disj_alg, since a map containing only cores joins with itself
-   but isn't a universal unit. *)
-Instance Global_Ghost {I} {RAs: I -> Ghost}: Ghost :=
-  { G := forall i, nat -> option (@G (RAs i)) }.
-
-Definition RA_of g := match g with GHOST RA _ _ => RA end.
-
-Definition Global_preds {I} (pds: I -> gname -> preds) :=
-  SomeP (PiType (ConstType I) (fun i => PiType (ConstType gname) (fun n =>
-    match pds i n with SomeP A _ => A end)))
-        (fun ts i n => match pds i n with SomeP A P => P ts end).
-  
-  
-  ArrowType (ConstType I) (ArrowType (ConstType gname) (PiType ())))
-    (fun ts i n => match pds i n with SomeP A P => P ts end).
-
-Definition own {I} `{EqDec I} {RAs: I -> Ghost} (n: gname) (a: ghost) {inG: {i | RAs i = RA_of a}} :=
-  match a with GHOST _ g (SomeP A pp) =>
-  EX A' : _, Own (GHOST Global_Ghost (fun j => if eq_dec j (proj1_sig inG) then fun m =>
-                                       if eq_dec m n then Some g else None else fun _ => None)
-                         (SomeP (ArrowType (ConstType I) (ArrowType (ConstType nat) Mpred))
-                                (fun _ => )) end.
-                 Print preds.
-
-Lemma ghost_alloc: forall {I} `{EqDec I} {RAs: I -> Ghost} {RA: Ghost} {inG: {i | RAs i = RA}}
-  (a: G) pp, (exists b, joins a b) ->
-  TT |-- bupd (EX g: gname, @own _ _ _ _ inG g a pp).
+Lemma Own_update: forall a b, ghost_fp_update a b ->
+  Own a |-- bupd (Own b).
 Proof.
+  intros; eapply derives_trans.
+  - apply (Own_update_ND a (Ensembles.Singleton _ b)).
+    repeat intro.
+    exists b; split; auto; constructor.
+  - apply bupd_mono.
+    apply exp_left; intro.
+    apply prop_andp_left; intro X; inv X; auto.
+Qed.
 
-Lemma ghost_op: forall {I} `{EqDec I} {RAs: I -> Ghost} {RA: Ghost} {inG: {i | RAs i = RA}}
-  (a b c: G) pp, join a b c ->
-  own g c = own g a * own g b.
+Lemma Own_unit: emp |-- EX a : _, !!(identity a) && Own a.
 Proof.
+  intros w ?; simpl in *.
+  exists (ghost_of w); split; [|split].
+  - apply ghost_of_identity; auto.
+  - intro; apply resource_at_identity; auto.
+  - rewrite ghost_of_approx; auto.
+Qed.
 
-Lemma ghost_valid: forall {I} `{EqDec I} {RAs: I -> Ghost} {RA: Ghost} {inG: {i | RAs i = RA}}
-  (a: G) pp, (exists b, joins a b) ->
-  TT |-- bupd (EX g: gname, @own _ _ _ _ inG g a pp).
+Definition gname := {I : Type & I * nat}%type.
+
+Definition singleton {A} k (x : A) : finmap A := repeat None k ++ Some x :: nil.
+
+Lemma singleton_get: forall {A} k (x : A) j,
+  finmap_get (singleton k x) j = if eq_dec j k then Some x else None.
 Proof.
+  intros; unfold finmap_get, singleton.
+  destruct (eq_dec j k).
+  - subst; rewrite app_nth2; rewrite repeat_length; [|omega].
+    rewrite minus_diag; auto.
+  - destruct (lt_dec j k).
+    + rewrite app_nth1 by (rewrite repeat_length; auto).
+      apply nth_repeat.
+    + rewrite app_nth2; rewrite repeat_length; [|omega].
+      destruct (j - k)%nat eqn: Hd; [omega|].
+      simpl; apply nth_nil.
+Qed.
 
-Lemma ghost_update: forall {I} `{EqDec I} {RAs: I -> Ghost} {RA: Ghost} {inG: {i | RAs i = RA}}
-  (a: G) pp, (exists b, joins a b) ->
-  TT |-- bupd (EX g: gname, @own _ _ _ _ inG g a pp).
+Program Definition single_ghost {I} {_ : EqDec I} {RAs} {RA} n {H: RAs (fst n) = RA} (a: @G RA) pp :=
+  GHOST I RAs (fun j => if eq_dec j (fst n) then
+                                singleton (snd n) _ else nil)
+         (fun j m => if eq_dec j (fst n) then if eq_dec m (snd n) then Some pp else None else None) _.
+Next Obligation.
 Proof.
+  intros; subst; auto.
+Defined.
+Next Obligation.
+Proof.
+  simpl; intros.
+  destruct (eq_dec _ _); [|discriminate].
+  destruct (eq_dec _ _); inv H1.
+  rewrite singleton_get, if_true; eauto.
+Qed.
 
+Definition own {RA: Ghost} (n: gname) (a: G) (pp: preds) :=
+  match n with existT A n =>
+    EX _ : EqDec A, EX RAs : _, EX H : RAs (fst n) = RA, Own (single_ghost(H := H) n a pp) end.
+
+(*Lemma fmap_alloc: forall f a,
+  fp_update_ND f (fun g => exists i, finmap_get f i = None /\ g = finmap_set f i a).*)
+
+(* Because the type of the ghost state is existentially quantified in the rmap, inG has to be a
+   state predicate instead of a pure assertion. *)
+Program Definition inG (RA: Ghost): pred rmap :=
+  (fun m => match ghost_of m with GHOST A RAs g _ _ =>
+    exists A_eq : EqDec A, exists inG : {i | RAs i = RA}, True end) && emp.
+Next Obligation.
+  repeat intro.
+  subst filtered_var program_branch_0; simpl in *.
+  lapply (age1_ghost_of _ _ H (ghost_of a)); [|symmetry; apply ghost_of_approx].
+  intros ->.
+  destruct (ghost_of a) eqn: Ha; auto.
+Qed.
+
+Lemma skipn_all: forall {A} (n : nat) (l : list A), (length l <= n)%nat -> skipn n l = nil.
+Proof.
+  induction n; destruct l; auto; simpl; intros; try omega.
+  apply IHn; omega.
+Qed.
+
+Opaque skipn.
+
+Lemma join_fresh: forall {A} {J: Join A} (m : finmap A) v,
+  join (singleton (fresh m) v) m (finmap_set m (fresh m) v).
+Proof.
+  intros; unfold singleton, finmap_set, fresh; simpl.
+  rewrite firstn_all, minus_diag, skipn_all by omega; simpl.
+  induction m; simpl; constructor; auto.
+  constructor.
+Qed.
+
+Lemma ghost_alloc: forall {RA: Ghost} a pp,
+  (exists b, joins a b) ->
+  inG RA |-- bupd (EX g: gname, own g a pp).
+Proof.
+  repeat intro; simpl in *.
+  destruct H1; inv H1.
+  rewrite <- H2 in H0.
+  destruct H0 as [(? & [i e] & _) Hemp].
+  eexists (ghost_approx (level a0) (GHOST _ RA0 (fun j => match eq_dec j i with
+    | left H => singleton (fresh (b j)) ((fun _ _ => _) e H) | _ => nil end)
+    (fun j n => if eq_dec j i then if eq_dec n (fresh (b j)) then Some pp
+                 else None else None) _)).
+  set (g' := ghost_approx _ _).
+  split.
+  - eexists; constructor.
+    + instantiate (1 := fun j => if eq_dec j i then _ else _).
+      hnf; intro j.
+      destruct (eq_dec _ _); [|constructor].
+      apply join_fresh.
+    + instantiate (1 := fun j n => if eq_dec j i then if eq_dec n (fresh (b j)) then _ else _ else _).
+      intros j n.
+      destruct (eq_dec _ _); [|constructor].
+      destruct (eq_dec _ _); [|constructor].
+      assert (pdsb j n = None) as ->; [|constructor].
+      destruct (pdsb j n) eqn: Hj; auto.
+      destruct (domb _ _ _ Hj) as [? Hget]; subst j n.
+      rewrite fresh_spec in Hget; discriminate.
+  - destruct (make_rmap (resource_at a0) g' (rmap_valid a0) (level a0)) as (m' & Hl & Hr & Hg).
+    { extensionality; apply resource_at_approx. }
+    { subst g'; rewrite ghost_fmap_fmap, !approx_oo_approx; auto. }
+    exists m'; repeat split; auto.
+    exists (existT _ A (i, fresh (b i))).
+    exists _, _, e; split; simpl.
+    + intro; rewrite Hr; apply resource_at_identity; auto.
+    + rewrite Hl, Hg; subst g'; apply ghost_ext.
+      * extensionality j.
+        destruct (eq_dec _ _); auto.
+        rewrite e0; auto.
+      * extensionality j n.
+        destruct (eq_dec _ _); subst; auto.
+  Unshelve.
+  simpl; intros.
+  destruct (eq_dec _ _); [|discriminate].
+  rewrite singleton_get.
+  destruct (eq_dec _ _); inv H0; eauto.
+  simpl; intros.
+  destruct (eq_dec _ _); [|eauto].
+  rewrite finmap_get_set.
+  destruct (eq_dec _ _); eauto.
+Qed.
+
+Lemma singleton_join: forall {A} {J: Join A} a b c k,
+  join (singleton k a) (singleton k b) (singleton k c) <-> join a b c.
+Proof.
+  unfold singleton; induction k; simpl.
+  - split.
+    + inversion 1; subst.
+      inv H3; auto.
+    + repeat constructor; auto.
+  - rewrite <- IHk.
+    split; [inversion 1 | repeat constructor]; auto.
+Qed.
+
+Lemma single_ghost_join: forall I (I_eq : EqDec I) (RAs: I -> Ghost) RA n
+  (H : RAs (fst n) = RA) a b c pp, join a b c ->
+  join (single_ghost(H := H) n a pp) (single_ghost(H := H) n b pp) (single_ghost(H := H) n c pp).
+Proof.
+  intros; constructor.
+  - intros i.
+    destruct (eq_dec _ _); [|constructor].
+    apply singleton_join; subst; auto.
+  - intros ??; destruct (eq_dec _ _); [|constructor].
+    destruct (eq_dec _ _); constructor; auto.
+Qed.
+
+Lemma ghost_op: forall {RA: Ghost} g (a1 a2 a3: G) pp,
+  join a1 a2 a3 ->
+  own g a3 pp = own g a1 pp * own g a2 pp.
+Proof.
+  intros; apply pred_ext.
+  - destruct g.
+    repeat (apply exp_left; intro).
+    erewrite Own_op by (apply single_ghost_join, H).
+    apply sepcon_derives; repeat eapply exp_right; eauto.
+  - destruct g.
+    intros ? (w1 & w2 & J & (? & ? & ? & ? & Hg1) & (? & ? & ? & ? & Hg2)).
+    pose proof (ghost_of_join _ _ _ J) as Jg.
+    rewrite Hg1, Hg2 in Jg; inversion Jg.
+    repeat inj_pair_tac.
+    do 3 eexists.
+    erewrite Own_op by (apply single_ghost_join, H).
+    exists w1, w2; repeat split; auto.
+    + simpl in *.
+      rewrite Hg1; apply ghost_ext.
+      * extensionality j.
+        destruct (eq_dec _ _), (eq_dec _ _); try contradiction; auto.
+        replace e with e0 by apply proof_irr; auto.
+      * extensionality i n.
+        destruct (eq_dec i _), (eq_dec i _); try contradiction; auto.
+    + simpl in *.
+      rewrite Hg2; apply ghost_ext; auto.
+      replace x5 with x2 by apply proof_irr; auto.
+Qed.
+
+Lemma singleton_join_inv: forall {A} {J: Join A} k a b c,
+  join (singleton k a) (singleton k b) c -> exists c', join a b c' /\ c = singleton k c'.
+Proof.
+  unfold singleton; induction k; inversion 1; subst.
+  - assert (m3 = nil) by (inv H6; auto).
+    inv H5; eauto.
+  - assert (a3 = None) by (inv H5; auto); subst.
+    edestruct IHk as (? & ? & ?); eauto; subst; eauto.
+Qed.
+
+Lemma ghost_conflict: forall {RA: Ghost} g (a1 a2: G) pp,
+  own g a1 pp * own g a2 pp |-- !!joins a1 a2.
+Proof.
+  intros.
+  destruct g as [? [i]]; intros w (? & ? & J & (? & ? & ? & ? & Hg1) & (? & ? & e1 & ? & Hg2)); simpl.
+  apply ghost_of_join in J.
+  rewrite Hg1, Hg2 in J; inv J.
+  repeat inj_pair_tac.
+  specialize (H3 i); simpl in *.
+  destruct (eq_dec i i); [|contradiction].
+  destruct (eq_dec i i); [|contradiction].
+  apply singleton_join_inv in H3 as (? & J & ?); clear - J.
+  rewrite (UIP_refl _ _ e), (UIP_refl _ _ e0), (UIP_refl _ _ e1) in J; eauto.
+Qed.
+
+Definition fp_update_ND {RA: Ghost} (a: G) B := forall c, joins a c -> exists b, B b /\ joins b c.
+
+Lemma singleton_join_some: forall {A} {J: Join A} k (a b c: A) m
+  (Hget: finmap_get m k = Some b) (Hjoin: join a b c),
+  join (singleton k a) m (finmap_set m k c).
+Proof.
+  unfold finmap_get; induction k; intros.
+  - destruct m; [rewrite nth_nil in Hget; discriminate|].
+    simpl in *; subst; repeat constructor; auto.
+  - destruct m; [discriminate|].
+    repeat constructor; eapply IHk; eauto.
+Qed.
+
+Lemma singleton_join_none: forall {A} {J: Join A} k (a: A) m (Hget: finmap_get m k = None),
+  join (singleton k a) m (finmap_set m k a).
+Proof.
+  unfold finmap_get; induction k; intros.
+  - destruct m; simpl in *; subst; repeat constructor.
+  - destruct m; repeat constructor; eapply IHk; eauto.
+Qed.
+
+Lemma ghost_update_ND: forall {RA: Ghost} g (a: G) B pp,
+  fp_update_ND a B -> own g a pp |-- bupd (EX b : _, !!(B b) && own g b pp).
+Proof.
+  intros.
+  destruct g as [? [i n]].
+  repeat (apply exp_left; intro).
+  eapply derives_trans.
+  - apply Own_update_ND with
+      (B := fun g => exists b, B b /\ g = @single_ghost _ _ _ _ (i, n) x2 b pp).
+    intros ?? [? J].
+    inv J; repeat inj_pair_tac.
+    pose proof (H6 i) as J.
+    apply finmap_get_join with (i0 := n) in J.
+    destruct (eq_dec i i); [|contradiction].
+    rewrite singleton_get, if_true in J by auto.
+    destruct (finmap_get (b0 i) n) eqn: Hb.
+    + destruct (finmap_get (c1 i) n); [|contradiction].
+      rewrite (UIP_refl _ _ e) in J.
+      lapply (H g); eauto.
+      intros (b & ? & [g' J']); simpl in *.
+      pose proof (singleton_join_some _ _ _ _ _ Hb J').
+      do 2 eexists; eauto.
+      eexists; constructor; eauto; simpl.
+      instantiate (1 := fun j => match eq_dec j i with
+        left H => finmap_set (b0 j) n (eq_rect_r (fun j => @G (x1 j)) g' H) | _ => b0 j end).
+      intro j; destruct (eq_dec j i); [|constructor].
+      subst; auto.
+    + lapply (H (core a)); [|eexists; apply join_comm, core_unit].
+      intros (b & ? & _).
+      do 2 eexists; eauto.
+      eexists; constructor; eauto; simpl.
+      instantiate (1 := fun j => match eq_dec j i with
+        left H => _ | _ => b0 j end).
+      intro j; destruct (eq_dec j i); [|constructor].
+      apply singleton_join_none; subst; auto.
+  - apply bupd_mono.
+    apply exp_left; intro; apply prop_andp_left; intros (? & ? & ?); subst.
+    eapply exp_right, andp_right; [repeat intro; simpl; eauto|].
+    repeat eapply exp_right; auto.
+  Unshelve.
+  intros j m ??; specialize (H7 j m); simpl in *.
+  destruct (eq_dec _ _); [|eapply domb; inv H7; rewrite H2 in *; eauto].
+  rewrite finmap_get_set; destruct (eq_dec _ _); eauto.
+  eapply domb; inv H7; rewrite H2 in *; eauto.
+  intros j m ??; specialize (H7 j m); simpl in *.
+  destruct (eq_dec _ _); [|eapply domb; inv H7; rewrite H1 in *; eauto].
+  rewrite finmap_get_set; destruct (eq_dec _ _); eauto.
+  eapply domb; inv H7; rewrite H1 in *; eauto.
+Qed.
+
+Definition fp_update {RA: Ghost} (a b : G) := forall c, joins a c -> joins b c.
+
+Lemma ghost_update: forall {RA: Ghost} g (a b: G) pp,
+  fp_update a b -> own g a pp |-- bupd (own g b pp).
+Proof.
+  intros; eapply derives_trans.
+  - apply (ghost_update_ND g a (Ensembles.Singleton _ b)).
+    intros ? J; destruct (H _ J).
+    do 2 eexists; [constructor | eauto].
+  - apply bupd_mono.
+    apply exp_left; intro; apply prop_andp_left; intro X; inv X; auto.
+Qed.
